Weidenbach_Book/WB_More_Refinement.thy
@@ -217,8 +217,11 @@ notation
   comp7 (infixl "\<circ>\<circ>\<circ>\<circ>\<circ>\<circ>" 55) and
   comp8 (infixl "\<circ>\<circ>\<circ>\<circ>\<circ>\<circ>\<circ>" 55)
 
+notation prod_assn (infixr "*a" 90)
+
 
 subsection \<open>More Theorems for Refinement\<close>
+
 
 lemma SPEC_add_information: \<open>P \<Longrightarrow> A \<le> SPEC Q \<Longrightarrow> A \<le> SPEC(\<lambda>x. Q x \<and> P)\<close>
   by auto
